***NO_CI*** some verification of dexor

secure_api/aead/Crypto.AEAD.EnxorDexor.fst
@@ -435,26 +435,50 @@ val counter_enxor:
     modifies_table_above_x_and_buffer t x cipher h0 h1 /\
     enxor_invariant t x len 0ul plain cipher h_init h1))
 #set-options "--z3rlimit 200 --initial_fuel 0 --max_fuel 0 --initial_ifuel 0 --max_ifuel 0"
-let rec counter_enxor #i t x len remaining_len plain cipher h_init =
+let counter_enxor #i t x len remaining_len plain cipher h_init =
   let completed_len = len -^ remaining_len in
   let h0 = get () in
-  if remaining_len <> 0ul then
-    begin // at least one more block
-      let starting_pos = len -^ remaining_len in
-      let l = min remaining_len (PRF.blocklen i) in
-      let cipher_hd = Buffer.sub cipher starting_pos l in
-      let plain_hd = Plain.sub plain starting_pos l in
-      PRF.prf_enxor i t x l cipher_hd plain_hd;
-      let h1 = get () in
-      x_buffer_1_modifies_table_above_x_and_buffer t x cipher h0 h1;
-      if safeMac i then prf_enxor_leaves_none_strictly_above_x t x len remaining_len cipher h0 h1;
-      extending_counter_blocks t x (v len) (v completed_len) plain cipher h0 h1 h_init;
-      let y = PRF.incr i x in
-      counter_enxor t y len (remaining_len -^ l) plain cipher h_init;
-      let h2 = get () in
-      trans_modifies_table_above_x_and_buffer t x y cipher h0 h1 h2
-    end
+  if remaining_len <> 0ul then begin // at least one more block
+    push_frame ();
+
+    let remaining = salloc #u32 #(Heap.trivial_preorder u32) remaining_len in
+    let prf_dom   = salloc #(PRF.domain i) #(Heap.trivial_preorder (PRF.domain i)) x in
+
+    let test :unit -> Stack bool (fun _ -> True) (fun _ _ _ -> True) = fun _ -> !remaining <> 0ul in
+    let body :unit -> Stack unit (fun _ -> True) (fun _ _ _ -> True)
+      = fun _ ->
+        let remaining_len = !remaining in
+	let x = !prf_dom in
+      
+        let starting_pos = len -^ remaining_len in
+        let l = min remaining_len (PRF.blocklen i) in
+        let cipher_hd = Buffer.sub cipher starting_pos l in
+        let plain_hd = Plain.sub plain starting_pos l in
+        PRF.prf_enxor i t x l cipher_hd plain_hd;
+
+        remaining := remaining_len -^ l;
+	prf_dom := PRF.incr i x
+    in
+
+    C.Loops.while test body;
+    pop_frame ()
+
+  end
   else refl_modifies_table_above_x_and_buffer t x cipher h0
+    //   let starting_pos = len -^ remaining_len in
+    //   let l = min remaining_len (PRF.blocklen i) in
+    //   let cipher_hd = Buffer.sub cipher starting_pos l in
+    //   let plain_hd = Plain.sub plain starting_pos l in
+    //   PRF.prf_enxor i t x l cipher_hd plain_hd;
+    //   let h1 = get () in
+    //   x_buffer_1_modifies_table_above_x_and_buffer t x cipher h0 h1;
+    //   if safeMac i then prf_enxor_leaves_none_strictly_above_x t x len remaining_len cipher h0 h1;
+    //   extending_counter_blocks t x (v len) (v completed_len) plain cipher h0 h1 h_init;
+    //   let y = PRF.incr i x in
+    //   counter_enxor t y len (remaining_len -^ l) plain cipher h_init;
+    //   let h2 = get () in
+    //   trans_modifies_table_above_x_and_buffer t x y cipher h0 h1 h2
+    // end
 
 (*+ enxor: The main function exposed to clients for encryption **)
 val enxor  :
@@ -785,37 +809,91 @@ val counter_dexor:
   ST unit (requires (fun h -> dexor_requires t x remaining_len plain cipher p h))
           (ensures (fun h0 _ h1 -> dexor_ensures t x plain cipher p h0 h1))
 #reset-options "--z3rlimit 200 --initial_fuel 0 --max_fuel 0 --initial_ifuel 0 --max_ifuel 0"
-let rec counter_dexor i t x len remaining_len plain cipher p =
-  let completed_len = len -^ remaining_len in
+let counter_dexor i t x len remaining_len plain cipher p =
   let h0 = get () in
   if safeId i then ST.recall (itable i t);
-  if remaining_len <> 0ul then
-    begin // at least one more block
-      let starting_pos = len -^ remaining_len in
-      let l = min remaining_len (PRF.blocklen i) in
-      let cipher_hd = Buffer.sub cipher starting_pos l in
-      let plain_hd = Plain.sub plain starting_pos l in
+  if remaining_len <> 0ul then begin
+    push_frame ();
 
-      invert_prf_contains_all_otp_blocks_st i x len remaining_len t p cipher h0;
-      prf_dexor i t x l cipher_hd plain_hd;
+    let remaining = salloc #u32 #(Heap.trivial_preorder u32) remaining_len in
+    let prf_dom   = salloc #(PRF.domain i) #(Heap.trivial_preorder (PRF.domain i)) x in
 
-      let h1 = get() in
-      let y = PRF.incr i x in
-      frame_prf_contains_all_otp_blocks_st x y (remaining_len -^ l) t plain p cipher h0 h1;
-      FStar.Classical.move_requires (FStar.Buffer.lemma_reveal_modifies_1 (as_buffer plain) h0) h1;
-      extend_decrypted_up_to t x remaining_len plain p cipher h0 h1;
-      incr_remaining_len_ok x len remaining_len;
+    let local_liveness (h:mem) = h `HS.contains` remaining /\ h `HS.contains` prf_dom /\
+                                 Buffer.disjoint_ref_2 (Plain.as_buffer plain) remaining prf_dom /\
+   			         Buffer.disjoint_ref_2 cipher remaining prf_dom
+    in
 
-      counter_dexor i t y len (remaining_len -^ l) plain cipher p;
+    let pre (h:mem) = local_liveness h /\ dexor_requires t (HS.sel h prf_dom) (HS.sel h remaining) plain cipher p h in
+    let post (b:bool) (h:mem) = b = (HS.sel h remaining <> 0ul) /\ local_liveness h /\ 
+                                dexor_requires t (HS.sel h prf_dom) (HS.sel h remaining) plain cipher p h
+    in
 
-      let h2 = get () in
-      dexor_of_prf_dexor_modifies t x plain_hd h0 h1;
-      dexor_modifies_widen t x plain starting_pos l h0 h1;
-      dexor_modifies_trans t x y plain h0 h1 h2;
-      FStar.Classical.move_requires (Buffer.lemma_reveal_modifies_1 (Plain.as_buffer plain) h0) h1;
-      FStar.Classical.move_requires (Buffer.lemma_reveal_modifies_1 (Plain.as_buffer plain) h1) h2
-    end
-   else dexor_modifies_refl t x plain h0
+    let test :unit -> Stack bool (fun h0 -> pre h0) (fun _ b h1  -> post b h1) = fun _ -> !remaining <> 0ul in
+
+    let body :unit -> Stack unit (fun h0 -> post true h0) (fun _ _ h1  -> pre h1)
+      = fun _ ->
+        let h0 = ST.get () in
+
+        let remaining_len = !remaining in
+        let x = !prf_dom in
+
+        let starting_pos = len -^ remaining_len in
+        let l = min remaining_len (PRF.blocklen i) in
+        let cipher_hd = Buffer.sub cipher starting_pos l in
+        let plain_hd = Plain.sub plain starting_pos l in
+
+        invert_prf_contains_all_otp_blocks_st i x len remaining_len t p cipher h0;
+        prf_dexor i t x l cipher_hd plain_hd;
+
+        let h1 = ST.get () in
+        incr_remaining_len_ok x len remaining_len;
+        frame_prf_contains_all_otp_blocks_st x (PRF.incr i x) (remaining_len -^ l) t plain p cipher h0 h1;
+        extend_decrypted_up_to t x remaining_len plain p cipher h0 h1;
+
+        remaining := remaining_len -^ l;
+        prf_dom := PRF.incr i x;
+
+        let h2 = ST.get () in
+        assert (dexor_requires t (PRF.incr i x) (remaining_len -^ l) plain cipher p h2);
+        assert (local_liveness h2);
+        assume (HyperStack.ST.equal_domains h0 h2)
+    in
+    admit ();
+    //F* crashes with h0 not found
+    C.Loops.while test body;
+    pop_frame ()
+  end
+  else dexor_modifies_refl t x plain h0
+
+  // let h0 = get () in
+  // if safeId i then ST.recall (itable i t);
+  // if remaining_len <> 0ul then
+  //   begin // at least one more block
+  //     let starting_pos = len -^ remaining_len in
+  //     let l = min remaining_len (PRF.blocklen i) in
+  //     let cipher_hd = Buffer.sub cipher starting_pos l in
+  //     let plain_hd = Plain.sub plain starting_pos l in
+
+  //     invert_prf_contains_all_otp_blocks_st i x len remaining_len t p cipher h0;
+  //     prf_dexor i t x l cipher_hd plain_hd;
+
+  //     let h1 = get() in
+  //     let y = PRF.incr i x in
+  //     frame_prf_contains_all_otp_blocks_st x y (remaining_len -^ l) t plain p cipher h0 h1;
+  //     FStar.Classical.move_requires (FStar.Buffer.lemma_reveal_modifies_1 (as_buffer plain) h0) h1;
+  //     extend_decrypted_up_to t x remaining_len plain p cipher h0 h1;
+  //     incr_remaining_len_ok x len remaining_len;
+
+  //     counter_dexor i t y len (remaining_len -^ l) plain cipher p;
+
+  //     let h2 = get () in
+  //     dexor_of_prf_dexor_modifies t x plain_hd h0 h1;
+  //     dexor_modifies_widen t x plain starting_pos l h0 h1;
+  //     dexor_modifies_trans t x y plain h0 h1 h2;
+  //     FStar.Classical.move_requires (Buffer.lemma_reveal_modifies_1 (Plain.as_buffer plain) h0) h1;
+  //     FStar.Classical.move_requires (Buffer.lemma_reveal_modifies_1 (Plain.as_buffer plain) h1) h2
+  //   end
+  //  else dexor_modifies_refl t x plain h0
 
 let decrypt_ok (#i:id) (n:Cipher.iv (Cipher.algi i)) (st:aead_state i Reader)
                (#aadlen:aadlen) (aad:lbuffer (v aadlen))
